De_Bruijn/named.ml
@@ -1,8 +1,15 @@
 (* ========================================================================= *)
 (* Named encoding of simple untyped lambda calculus.                         *)
-(* Inspired by Harrison's "HOL in HOL"                                       *)
+(* Partially inspired by Harrison's "HOL in HOL"                             *)
 (* (folder Model in the HOL Light distribution).                             *)
 (* ========================================================================= *)
+
+type_invention_warning := false;;
+needs "Library/rstc.ml";;
+type_invention_warning := true;;
+
+needs "De_Bruijn/misc.ml";;
+needs "De_Bruijn/lib.ml";;
 
 let term_INDUCT,term_RECUR = define_type
   "term = Var num
@@ -12,15 +19,6 @@ let term_INDUCT,term_RECUR = define_type
 let term_INJ = injectivity "term";;
 let term_DISTINCT = distinctness "term";;
 let term_CASES = cases "term";;
-
-let FVARS_RULES,FVARS_INDUCT,FVARS_CASES = new_inductive_set
-  `(!x. x IN FVARS (Var x)) /\
-   (!x s t. x IN FVARS s ==> x IN FVARS (Comb s t)) /\
-   (!x s t. x IN FVARS t ==> x IN FVARS (Comb s t)) /\
-   (!x y t. ~(x = y) /\ x IN FVARS t ==> x IN FVARS (Lam y t))`;;
-
-(* let ALPHA_RULES,ALPHA_INDUCT,ALPHA_CASES = new_inductive_definition
-  `(x,y) IN R ==> ALPHA R (Var x) (Var y)`;; *)
 
 (* ------------------------------------------------------------------------- *)
 (* Alpha-conversion.                                                         *)
@@ -43,20 +41,218 @@ let RACONV_RULES,RACONV_INDUCT,RACONV_CASES = new_inductive_definition
      RACONV (CONS (x,y) env) (s,t) ==> RACONV env (Lam x s,Lam y t))`;;
 
 let RACONV = prove
- (`(RACONV env (Var x1,Var x2) <=> ALPHAVARS env (x1,x2)) /\
-   (RACONV env (Var x1,Comb l2 r2) <=> F) /\
-   (RACONV env (Var x1,Lam x2 t2) <=> F) /\
-   (RACONV env (Comb l1 r1,Var x2) <=> F) /\
-   (RACONV env (Comb l1 r1,Comb l2 r2) <=>
-        RACONV env (l1,l2) /\ RACONV env (r1,r2)) /\
-   (RACONV env (Comb l1 r1,Lam x2 t2) <=> F) /\
-   (RACONV env (Lam x1 t1,Var x2) <=> F) /\
-   (RACONV env (Lam x1 t1,Comb l2 r2) <=> F) /\
-   (RACONV env (Lam x1 t1,Lam x2 t2) <=>
-        RACONV (CONS (x1,x2) env) (t1,t2))`,
-  REPEAT CONJ_TAC THEN
-  GEN_REWRITE_TAC LAND_CONV [RACONV_CASES] THEN
+ (`RACONV env (Var x1,Var x2) = ALPHAVARS env (x1,x2) /\
+   RACONV env (Var x1,Comb l2 r2) = F /\
+   RACONV env (Var x1,Lam x2 t2) = F /\
+   RACONV env (Comb l1 r1,Var x2) = F /\
+   RACONV env (Comb l1 r1,Comb l2 r2) =
+     (RACONV env (l1,l2) /\ RACONV env (r1,r2)) /\
+   RACONV env (Comb l1 r1,Lam x2 t2) = F /\
+   RACONV env (Lam x1 t1,Var x2) = F /\
+   RACONV env (Lam x1 t1,Comb l2 r2) = F /\
+   RACONV env (Lam x1 t1,Lam x2 t2) = RACONV (CONS (x1,x2) env) (t1,t2)`,
+  REPEAT CONJ_TAC THEN GEN_REWRITE_TAC LAND_CONV [RACONV_CASES] THEN
   REWRITE_TAC[term_INJ; term_DISTINCT; PAIR_EQ] THEN MESON_TAC[]);;
 
 let ACONV = new_definition
  `ACONV t1 t2 <=> RACONV [] (t1,t2)`;;
+
+(* ------------------------------------------------------------------------- *)
+(* Reflexivity of alpha-conversion.                                          *)
+(* ------------------------------------------------------------------------- *)
+
+let ALPHAVARS_REFL = prove
+ (`!env t. ALL (\(s,t). s = t) env ==> ALPHAVARS env (t,t)`,
+  MATCH_MP_TAC list_INDUCT THEN REWRITE_TAC[ALL; ALPHAVARS] THEN
+  REWRITE_TAC[FORALL_PAIR_THM] THEN
+  CONV_TAC(ONCE_DEPTH_CONV GEN_BETA_CONV) THEN MESON_TAC[PAIR_EQ]);;
+
+let RACONV_REFL = prove
+ (`!t env. ALL (\(s,t). s = t) env ==> RACONV env (t,t)`,
+  MATCH_MP_TAC term_INDUCT THEN REWRITE_TAC[RACONV] THEN REPEAT STRIP_TAC THENL
+  [ASM_SIMP_TAC[ALPHAVARS_REFL];
+   ASM_MESON_TAC[];
+   ASM_MESON_TAC[];
+   FIRST_X_ASSUM MATCH_MP_TAC THEN ASM_REWRITE_TAC[ALL]]);;
+
+let ACONV_REFL = prove
+ (`!t. ACONV t t`,
+  REWRITE_TAC[ACONV] THEN SIMP_TAC[RACONV_REFL; ALL]);;
+
+(* ------------------------------------------------------------------------- *)
+(* Free variables.                                                           *)
+(* ------------------------------------------------------------------------- *)
+
+let FVARS_RULES,FVARS_INDUCT,FVARS_CASES = new_inductive_set
+  `(!x. x IN FVARS (Var x)) /\
+   (!x s t. x IN FVARS s ==> x IN FVARS (Comb s t)) /\
+   (!x s t. x IN FVARS t ==> x IN FVARS (Comb s t)) /\
+   (!x y t. ~(x = y) /\ x IN FVARS t ==> x IN FVARS (Lam y t))`;;
+
+let FVARS_INVERSION = prove
+ (`(!x y. x IN FVARS (Var y) <=> x = y) /\
+   (!x s t. x IN FVARS (Comb s t) <=> x IN FVARS s \/ x IN FVARS t) /\
+   (!x y t. x IN FVARS (Lam y t) <=> ~(x = y) /\ x IN FVARS t)`,
+  REPEAT STRIP_TAC THEN GEN_REWRITE_TAC LAND_CONV [FVARS_CASES] THEN
+  REWRITE_TAC[term_DISTINCT; term_INJ] THEN MESON_TAC[]);;
+
+let FVARS_CLAUSES = prove
+ (`FVARS (Var x) = {x} /\
+   FVARS (Comb s t) = FVARS s UNION FVARS t /\
+   FVARS (Lam x t) = FVARS t DELETE x`,
+  REWRITE_TAC[EXTENSION; FVARS_INVERSION] THEN SET_TAC[]);;
+
+let ALPHAVARS_EQ = prove
+ (`!env x x' y y':A. ALPHAVARS env (x,y) /\ ALPHAVARS env (x',y')
+                     ==> (x = x' <=> y = y')`,
+  LIST_INDUCT_TAC THEN REWRITE_TAC[ALPHAVARS] THENL [MESON_TAC[]; ALL_TAC] THEN
+  STRUCT_CASES_TAC (ISPEC `h:A#A` PAIR_SURJECTIVE) THEN
+  REWRITE_TAC[PAIR_EQ] THEN ASM_MESON_TAC[]);;
+
+let FVARS_RACONV = prove
+ (`!env p. RACONV env p
+           ==> (!x. x IN FVARS (FST p) /\ ~(?y. MEM (x,y) env) <=>
+                    x IN FVARS (SND p) /\ ~(?y. MEM (y,x) env))`,
+  MATCH_MP_TAC RACONV_INDUCT THEN
+  REWRITE_TAC[FVARS_INVERSION; MEM; PAIR_EQ] THEN CONJ_TAC THENL
+  [LIST_INDUCT_TAC THEN REWRITE_TAC[ALPHAVARS; MEM] THENL
+   [MESON_TAC[];
+    STRUCT_CASES_TAC (ISPEC `h:num#num` PAIR_SURJECTIVE) THEN
+    REWRITE_TAC[PAIR_EQ] THEN ASM_MESON_TAC[]];
+   MESON_TAC[]]);;
+
+let VFARS_ACONV = prove
+ (`!s t x. ACONV s t ==> (x IN FVARS s <=> x IN FVARS t)`,
+  REPEAT GEN_TAC THEN REWRITE_TAC[ACONV] THEN
+  DISCH_THEN(MP_TAC o MATCH_MP FVARS_RACONV) THEN
+  SIMP_TAC[MEM; FST; SND]);;
+
+(* ------------------------------------------------------------------------- *)
+(* Variant function. Deliberately underspecified at the moment. In a bid to  *)
+(* expunge use of sets, just pick it distinct from what's free in a term.    *)
+(* ------------------------------------------------------------------------- *)
+
+let FINITE_FVARS = prove
+ (`!t. FINITE (FVARS t)`,
+  MATCH_MP_TAC term_INDUCT THEN
+  REWRITE_TAC[FVARS_CLAUSES; FINITE_SING; FINITE_UNION; FINITE_DELETE]);;
+
+let AVOID_FINITE_EXISTS = prove
+ (`!s:A->bool. INFINITE (:A) /\ FINITE s ==> ?x. ~(x IN s)`,
+  GEN_TAC THEN STRIP_TAC THEN
+  SUBGOAL_THEN `~((:A) DIFF s= {})` (fun th -> SET_TAC[th]) THEN
+  MATCH_MP_TAC INFINITE_NONEMPTY THEN ASM_SIMP_TAC[INFINITE_DIFF_FINITE]);;
+
+let FRESH = (specify o prove)
+ (`!s:num->bool. FINITE s ==> ?FRESH. ~(FRESH IN s)`,
+  MESON_TAC[AVOID_FINITE_EXISTS; num_INFINITE]);;
+
+(* ------------------------------------------------------------------------- *)
+(* Term substitution.                                                        *)
+(* ------------------------------------------------------------------------- *)
+
+let VSUBST = define
+  `(!f x. VSUBST f (Var x) = f x) /\
+   (!f s t. VSUBST f (Comb s t) = Comb (VSUBST f s) (VSUBST f t)) /\
+   (!f x t. VSUBST f (Lam x t) =
+            let x' = FRESH (UNIONS {FVARS (f y) | y IN FVARS t}) in
+            Lam x' (VSUBST (\v. if v = x then Var x' else f v) t))`;;
+
+let IN_FVARS_VSUBST = prove
+ (`!t u f. u IN FVARS (VSUBST f t) <=>
+           ?y. y IN FVARS t /\ u IN FVARS (f y)`,
+  MATCH_MP_TAC term_INDUCT THEN REPEAT STRIP_TAC THEN
+  ASM_REWRITE_TAC[VSUBST; FVARS_INVERSION] THENL
+  [REWRITE_TAC[UNWIND_THM2]; MESON_TAC[]; ALL_TAC] THEN
+  LET_TAC THEN ASM_REWRITE_TAC[FVARS_INVERSION] THEN EQ_TAC THENL
+  [STRIP_TAC THEN POP_ASSUM MP_TAC THEN COND_CASES_TAC THENL
+   [POP_ASSUM (SUBST_VAR_TAC o GSYM); ASM_REWRITE_TAC[]] THEN
+   ASM_REWRITE_TAC[FVARS_INVERSION] THEN ASM_MESON_TAC[];
+   ALL_TAC] THEN
+  STRIP_TAC THEN CONJ_TAC THENL [ALL_TAC; ASM_MESON_TAC[FVARS_INVERSION]] THEN
+  SUBGOAL_THEN `u IN UNIONS {FVARS (f y) | y IN FVARS a1} /\
+                ~(x' IN UNIONS {FVARS (f y) | y IN FVARS a1})`
+               (fun th -> MESON_TAC[th]) THEN
+  FIRST_X_ASSUM SUBST_VAR_TAC THEN CONJ_TAC THENL
+  [ASM SET_TAC []; MATCH_MP_TAC FRESH] THEN
+  REWRITE_TAC[FINITE_UNIONS; FORALL_IN_GSPEC; FINITE_FVARS] THEN
+  SUBGOAL_THEN
+    `!f t. {FVARS (f y) | y IN FVARS t} = IMAGE (FVARS o f) (FVARS t)`
+    (fun th -> REWRITE_TAC[th]) THENL
+  [REWRITE_TAC[IMAGE_o] THEN SET_TAC[];
+   MATCH_MP_TAC FINITE_IMAGE THEN REWRITE_TAC[FINITE_FVARS]]);;
+
+let FVARS_VSUBST = prove
+ (`!t f. FVARS (VSUBST f t) = UNIONS (IMAGE (FVARS o f) (FVARS t))`,
+  REWRITE_TAC[IMAGE_o; IN_FVARS_VSUBST; EXTENSION] THEN SET_TAC[]);;
+
+let ALPHAVARS_IMP_EQ = prove
+ (`!env x y:A. ALPHAVARS env (x,y) /\
+               (~(?y. MEM (x,y) env) \/ ~(?x. MEM (x,y) env))
+               ==> x = y`,
+  LIST_INDUCT_TAC THEN REWRITE_TAC[ALPHAVARS; MEM] THEN
+  STRUCT_CASES_TAC (ISPEC `h:A#A` PAIR_SURJECTIVE) THEN
+  REWRITE_TAC[PAIR_EQ] THEN ASM_MESON_TAC[]);;
+
+let RACONV_ENV_INDEPENDENT = prove
+ (`!env1 env2 s t.
+     (!x y. x IN FVARS s /\ y IN FVARS t
+            ==> (ALPHAVARS env1 (x,y) <=> ALPHAVARS env2 (x,y)))
+     ==> (RACONV env1 (s,t) <=> RACONV env2 (s,t))`,
+  SUBGOAL_THEN
+    `!env p. RACONV env p
+             ==> !env'. (!x y. x IN FVARS (FST p) /\ y IN FVARS (SND p)
+                               ==> (ALPHAVARS env (x,y) <=>
+                                    ALPHAVARS env' (x,y)))
+                        ==> RACONV env' p`
+      (fun th -> MESON_TAC[REWRITE_RULE[FORALL_PAIR_THM] th]) THEN
+  MATCH_MP_TAC RACONV_INDUCT THEN REWRITE_TAC[FVARS_INVERSION; RACONV] THEN
+  REPEAT CONJ_TAC THENL [MESON_TAC[]; MESON_TAC[]; ALL_TAC] THEN
+  REWRITE_TAC[ALPHAVARS; PAIR_EQ] THEN REPEAT STRIP_TAC THEN
+  FIRST_X_ASSUM MATCH_MP_TAC THEN REWRITE_TAC[ALPHAVARS; PAIR_EQ] THEN
+  ASM_MESON_TAC[]);;
+
+let SWAP = new_definition
+  `SWAP (x:A,y:B) = (y,x)`;;
+
+let REV_ASSOCD = define
+  `(REV_ASSOCD a [] d = d) /\
+   (REV_ASSOCD a (CONS (x,y) t) d =
+        if y = a then x else REV_ASSOCD a t d)`;;
+
+let ASSOCD = define
+  `(ASSOCD a [] d = d) /\
+   (ASSOCD a (CONS (x,y) t) d =
+        if x = a then y else ASSOCD a t d)`;;
+
+let ACONV_COMB = prove
+ (`!s1 s2 t1 t2. ACONV (Comb s1 t1) (Comb s2 t2) <=>
+                 ACONV s1 s2 /\ ACONV t1 t2`,
+  REWRITE_TAC[ACONV; RACONV]);;
+
+(*
+let RACONV_VSUBST = prove
+ (`!env s t f g.
+     RACONV env (s,t) /\
+     (!x y. ALPHAVARS env (x,y) /\ (~MEM (x,y) env ==> x IN FVARS s)
+            ==> RACONV env (f x,g y))
+     ==> RACONV env (VSUBST f s,VSUBST g t)`,
+
+  SUBGOAL_THEN
+    `!env p. RACONV env p
+             ==> !f g. (!x y. ALPHAVARS env (x,y) /\
+                             (~MEM (x,y) env ==> x IN FVARS (FST p))
+                             ==> RACONV env (f x,g y))
+                       ==> RACONV env (VSUBST f (FST p),VSUBST g (SND p))`
+    (fun th -> MESON_TAC[REWRITE_RULE[FORALL_PAIR_THM] th]) THEN
+*)
+
+(* 
+let ACONV_VSUBST = prove
+ (`!s t f g. ACONV s t /\ (!x. x IN FVARS s ==> ACONV (f x) (g x))
+             ==> ACONV (VSUBST f s) (VSUBST g t)`,
+
+REWRITE_TAC[ACONV]
+
+ );;
+*)
